CC/StoreContext/Lookup.lean
@@ -1,0 +1,35 @@
+import Mathlib.Data.Finset.Basic
+import Mathlib.Data.Finset.Image
+
+import CC.Basic
+import CC.Rename
+
+import CC.CaptureSet
+import CC.Context
+import CC.Term
+import CC.Type
+import CC.Typed
+import CC.Typed.Basic
+import CC.Typed.Rename
+import CC.EvalContext
+import CC.StoreContext.Basic
+import CC.Typed.CanonicalForm
+
+namespace CC
+
+theorem lookup_fun
+  (hs : TypedStore γ Γ)
+  (hx : Typed Γ (Term.var x) Cx (CType.capt Cf (PType.arr T U)))
+  (hl : LookupStore γ x ⟨Term.abs T' t, hval⟩) :
+  ∃ C0, Typed (Ctx.extend_var Γ T) t C0 U := by
+  have h1 := Typed.var_typing_bound hx
+  let ⟨C1, S1, hb, hsub⟩ := h1
+  have h2 := lookup_store_typing hs hb hl
+  let ⟨C2, ht⟩ := h2
+  simp at ht
+  apply Typed.cf_fun
+  apply Typed.sub
+  exact ht
+  constructor
+  apply Subcapt.refl
+  exact hsub
